Q4

NJ.v
@@ -1,6 +1,5 @@
-Require Import List.
-Import ListNotations.
 Require Import Arith.
+Require Import Lists.List.
 Require Import Coq.Relations.Relations.
 Require Coq.Vectors.Vector.
 Import Vector.VectorNotations.
@@ -11,7 +10,7 @@ Require Import Coq.Structures.Orders.
 Require Import Program.
 
 Hint Immediate eq_nat_dec.
-     
+
 Tactic Notation "solve_by_inversion_step" tactic(t) :=
   match goal with
     | H : _ |- _ => solve [ inversion H; subst; t ]
@@ -27,17 +26,17 @@ Tactic Notation "solve" "by" "inversion" "3" :=
 Tactic Notation "solve" "by" "inversion" :=
   solve by inversion 1.
 
-Ltac simpl_exist :=
-  repeat match goal with
-           | [ H : existT _ _ _ = existT _ _ _ |- _] => apply inj_pair2_eq_dec in H; eauto
-         end
-.
+Theorem Forall_app : forall A (R : A -> Prop) l1 l2,
+                       Forall R l1 -> Forall R l2 -> Forall R (l1 ++ l2).
+Proof.
+  induction l1; simpl; intros.
+  auto.
+  inversion H; constructor; auto.
+Qed.
 
-Ltac simpl_forall_list :=
-  repeat match goal with
-           | [ H : Forall _ ?l |- _ ] => is_list_constr l; inversion_clear H
-           | _ => idtac
-         end.
+Notation "'sigma' x .. y ',' p" := (sigT (fun x => .. (sigT (fun y => p)) ..))
+                                     (at level 180, x binder, right associativity)
+                                   : type_scope.
 
 Lemma fin_case :
   forall n (P : Fin.t (S n) -> Type),
@@ -83,6 +82,58 @@ Ltac finite :=
     | [ |- forall (x : Fin.t ?n), _ ] =>
       intros x; finite' n x
   end.
+
+Lemma eq_fin_dec : forall {n} (f f' : Fin.t n), {f = f'} + {f <> f'}.
+Proof.
+  induction n; intros.
+  apply Fin.case0; auto.
+  fin_dep_destruct f; fin_dep_destruct f';
+  try (right; intro; solve by inversion).
+  left; auto.
+  specialize (IHn x x0).
+  destruct IHn.
+  left; f_equal; auto.
+  right. intro. inversion H. apply inj_pair2_eq_dec in H1. auto. auto.
+Qed.
+
+Hint Immediate eq_fin_dec.
+
+Lemma eq_vector_dec_ind : forall {n A} (v v' : Vector.t A n), (forall i t, {v[@i] = t} + {v[@i] <> t}) -> {v = v'} + {v <> v'}.
+Proof.
+  induction n; dependent destruction v; dependent destruction v'; intros.
+  left; auto.
+  assert (forall (i : Fin.t n) (t : A), {v[@i] = t} + {v[@i] <> t}).
+  intros.
+  specialize (X (Fin.FS i) t); auto.
+  specialize (IHn _ v v' X0).
+  specialize (X Fin.F1 h0); simpl in X.
+  destruct IHn; destruct X; subst;
+  try (left; auto; fail).
+  right; intro; inversion H; auto.
+  right; intro; inversion H; auto; apply inj_pair2_eq_dec in H1; auto.
+  right; intro; inversion H; auto; apply inj_pair2_eq_dec in H1; auto.
+Qed.
+
+Lemma eq_vector_dec : forall {n A} (P : forall (t t' : A), {t = t'} + {t <> t'}) (v v' : Vector.t A n), {v = v'} + {v <> v'}.
+Proof.
+  intros. apply eq_vector_dec_ind.
+  intros. apply P.
+Qed.
+
+Hint Immediate eq_vector_dec.
+
+Lemma vector_map_inj : forall {n A B} (f : A -> B) (v v' : Vector.t A n)
+                       (P : forall i t', f v[@i] = f t' -> v[@i] = t'),
+                         Vector.map f v = Vector.map f v' -> v = v'.
+Proof.
+  induction v; intros; dependent destruction v'; auto.
+  intros. f_equal. 
+  inversion H. specialize (P Fin.F1 h0). auto.
+  assert (forall (i : Fin.t n) (t' : A), f v[@i] = f t' -> v[@i] = t').
+  intros. specialize (P (Fin.FS i) t'). simpl in P. auto.
+  specialize (IHv v' H0).
+  inversion H. apply inj_pair2_eq_dec in H3; auto.
+Qed.
 
 Lemma fin_compare : forall {n}, Fin.t n -> Fin.t n -> comparison.
 Proof.
@@ -136,8 +187,29 @@ Proof with eauto.
   destruct (fin_subst t x y) eqn:H2; inversion H; inversion H1; subst...
 Qed.
 
+Ltac simpl_exist :=
+  repeat (
+      repeat match goal with
+               | [ H : existT _ _ _ = existT _ _ _ |- _] =>
+                 (apply inj_pair2_eq_dec in H; [|eauto using eq_vector_dec; fail])
+               | [ H : existT _ _ _ = existT _ _ _, _ : existT _ _ _ = existT _ _ _ |- _] =>
+                 (apply inj_pair2_eq_dec in H; [|eauto using eq_vector_dec; fail])
+               | [ H : existT _ _ _ = existT _ _ _, _ : existT _ _ _ = existT _ _ _, _ : existT _ _ _ = existT _ _ _ |- _] =>
+                 (apply inj_pair2_eq_dec in H; [|eauto using eq_vector_dec; fail])
+             end;
+      subst; clear_dups
+    ).
+
+Ltac simpl_forall_list :=
+  repeat match goal with
+           | [ H : Forall _ ?l |- _ ] => is_list_constr l; inversion_clear H
+           | _ => idtac
+         end.
+
 Module Type TermDef.
   Parameter symbol : Type.
+  Parameter eq_symbol_dec : forall (s s' : symbol), {s = s'} + {s <> s'}.
+  Hint Immediate eq_symbol_dec.
   Parameter arity : symbol -> nat.
 End TermDef.
 
@@ -149,7 +221,7 @@ Module Expr (T : TermDef).
   | t_var : forall {n}, Fin.t n -> term n
   | t_term : forall {n} (s : symbol), Vector.t (term n) (arity s) -> term n
   .
-    
+  
   Definition termRect :=
       fun (P : forall n : nat, term n -> Type)
           (f : forall (n : nat) (t : Fin.t n), P n (@t_var n t))
@@ -161,11 +233,40 @@ Module Expr (T : TermDef).
       | t_term n0 s t0 => f0 n0 s t0 (fun i => F n0 (Vector.nth t0 i))
     end.
 
+  Theorem eq_term_dec : forall {n} (t t' : term n), {t = t'} + {t <> t'}.
+  Proof.
+    intro. induction t using termRect; intros;
+    destruct t'; try (right; intro; solve by inversion).
+    assert (H := eq_fin_dec t t0).
+    destruct H; subst.
+    left; auto.
+    right; intro; inversion H; simpl_exist; auto.
+    assert (H := eq_symbol_dec s s0).
+    destruct H; subst.
+    assert (H := eq_vector_dec_ind t t0 X).
+    destruct H; subst.
+    left; auto.
+    right; intro; inversion H; simpl_exist; auto.
+    right; intro; inversion H; simpl_exist; auto.
+  Qed.
+
+  Hint Immediate eq_term_dec.
+
   Fixpoint lift_term {n} (t : term n) : term (S n) :=
     match t with
       | t_var _ i => t_var (Fin.R 1 i)
       | t_term _ s ts => t_term s (Vector.map lift_term ts)
     end.
+
+  Theorem lift_term_inj : forall {n} (t t' : term n),
+                            lift_term t = lift_term t' -> t = t'.
+  Proof.
+    induction t using termRect; intros t' H0; destruct t';
+    simpl in H0; try (solve by inversion); inversion H0; simpl_exist; auto.
+    apply vector_map_inj in H3; subst; auto.
+  Qed.
+
+  Hint Immediate lift_term_inj.
 
   Inductive type : nat -> Type :=
   | ty_term : forall {n : nat}, term n -> type n
@@ -177,6 +278,70 @@ Module Expr (T : TermDef).
   | ty_top : forall {n : nat}, type n
   | ty_pair : forall {n : nat}, type n -> type n -> type n
   .
+
+  Ltac lift_dec_eq :=
+    match goal with
+      | [ |- { ?a ?b = ?a ?b' } + { ?a ?b <> ?a ?b' } ] =>
+        let H := fresh "H" in
+        let H0 := fresh "H" in
+        assert (H : {b = b'} + {b <> b'});
+          [ auto
+          | destruct H;
+            [ left; subst; auto
+            | right; unfold not; intros H0; inversion H0; simpl_exist; auto
+            ]
+          ]
+      | [ |- { ?a ?b ?c = ?a ?b' ?c' } + { ?a ?b ?c <> ?a ?b' ?c' } ] =>
+        let H := fresh "H" in
+        let H0 := fresh "H" in
+        let H1 := fresh "H" in
+        assert (H : {b = b'} + {b <> b'});
+          [ auto
+          | assert (H0 : {c = c'} + {c <> c'});
+            [ auto
+            | destruct H;
+              [ destruct H0;
+                [ left; subst; auto
+                | right; unfold not; intros H1; inversion H1; simpl_exist; auto
+                ]
+              | right; unfold not; intros H1; inversion H1; simpl_exist; auto
+              ]
+            ]
+          ]
+      | [ |- { ?a ?b ?c ?d = ?a ?b' ?c' ?d' } + { ?a ?b ?c ?d <> ?a ?b' ?c' ?d' } ] =>
+        let H := fresh "H" in
+        let H0 := fresh "H" in
+        let H1 := fresh "H" in
+        let H2 := fresh "H" in
+        assert (H : {b = b'} + {b <> b'});
+          [ auto
+          | assert (H0 : {c = c'} + {c <> c'});
+            [ auto
+            | assert (H1 : {d = d'} + {d <> d'});
+              [ auto
+              | destruct H;
+                [ destruct H0;
+                  [ destruct H1;
+                    [ left; subst; auto
+                    | right; unfold not; intros H2; inversion H2; simpl_exist; auto
+                    ]
+                  | right; unfold not; intros H2; inversion H2; simpl_exist; auto
+                  ]
+                | right; unfold not; intros H2; inversion H2; simpl_exist; auto
+                ]
+              ]
+            ]
+          ]
+    end.
+
+  Theorem eq_type_dec : forall {n} (t t' : type n), {t = t'} + {t <> t'}.
+  Proof.
+    intro. induction t; destruct t';
+           try (right; intro; solve by inversion);
+           try (lift_dec_eq).
+  Qed.
+
+  Hint Immediate eq_type_dec.
   
   Fixpoint lift_type {n} (t : type n) : type (S n) :=
   match t with
@@ -190,6 +355,14 @@ Module Expr (T : TermDef).
     | ty_top _ => ty_top
   end.
 
+  Theorem lift_type_inj : forall {n} (t t' : type n),
+                            lift_type t = lift_type t' -> t = t'.
+  Proof.
+    induction t; intros t' H; dependent destruction t'; inversion H; simpl_exist; f_equal; auto.
+  Qed.
+
+  Hint Immediate lift_type_inj.
+  
   Fixpoint term_subst {n} (i : Fin.t (S n)) (t : term n) (u : term (S n)) : term n :=
     match u as u' in term n' return forall pf : n' = S n,
                                       term n
@@ -225,7 +398,7 @@ Module Expr (T : TermDef).
     | e_exists : forall {n m : nat}, term m -> exp n m -> exp n m
     | e_ecase : forall {n m : nat}, exp n m -> exp (S n) (S m) -> exp n m
     | e_abs : forall {n m : nat}, exp (S n) m -> exp n m
-    | e_tapp : forall {n m : nat}, exp n (S m) -> term m -> exp n m
+    | e_tapp : forall {n m : nat}, exp n m -> term m -> exp n m
     | e_absurd : forall {n m}, exp n m -> exp n m
     | e_copair1 : forall {n m}, exp n m -> exp n m
     | e_copair2 : forall {n m}, exp n m -> exp n m
@@ -235,6 +408,16 @@ Module Expr (T : TermDef).
     | e_pair1 : forall {n m}, exp n m -> exp n m
     | e_pair2 : forall {n m}, exp n m -> exp n m
     .
+
+    Theorem eq_exp_dec : forall {n m} (e e' : exp n m), {e = e'} + {e <> e'}.
+    Proof.
+      intros n m. induction e; destruct e';
+                  try (right; intro; solve by inversion);
+                  try (lift_dec_eq).
+    Qed.
+    
+    Hint Immediate eq_exp_dec.
+  
 
   Definition sub_exp {n m} (t : exp n m) : list (exp n m) :=
   match t with
@@ -293,7 +476,6 @@ Module Expr (T : TermDef).
     | e_pair2 _ _ a => e_pair2 (lift_exp a)
   end.
 
-
     Fixpoint exp_subst {n m} (i : Fin.t (S n)) (t : exp n m) (u : exp (S n) m) : exp n m :=
       let eq_rect_exp {n m n' m'} (pf : n' = S n) (pf' : m' = m) x :=
           eq_rect n' (fun i => exp i m) (eq_rect m' (fun i => exp n' i) x _ pf') _ pf
@@ -312,7 +494,7 @@ Module Expr (T : TermDef).
         | e_exists _ m' a b => fun pf pf' => e_exists (eq_rect m' term a _ pf') (exp_subst i t (eq_rect_exp pf pf' b))
         | e_ecase _ _ a b => fun pf pf' => e_ecase (exp_subst i t (eq_rect_exp pf pf' a)) (exp_subst (Fin.FS i) (lift_exp_n (lift_exp t)) (eq_rect_exp (f_equal S pf) (f_equal S pf') b))
         | e_abs _ _ a => fun pf pf' => e_abs (exp_subst (Fin.FS i) (lift_exp_n t) (eq_rect_exp (f_equal S pf) pf' a))
-        | e_tapp _ _ a b => fun pf pf' => e_tapp (exp_subst i (lift_exp t) (eq_rect_exp pf (f_equal S pf') a)) (eq_rect _ _ b _ pf')
+        | e_tapp _ _ a b => fun pf pf' => e_tapp (exp_subst i t (eq_rect_exp pf pf' a)) (eq_rect _ _ b _ pf')
         | e_absurd _ _ a => fun pf pf' => e_absurd (exp_subst i t (eq_rect_exp pf pf' a))
         | e_copair1 _ _ a => fun pf pf' => e_copair1 (exp_subst i t (eq_rect_exp pf pf' a))
         | e_copair2 _ _ a => fun pf pf' => e_copair2 (exp_subst i t (eq_rect_exp pf pf' a))
@@ -325,30 +507,43 @@ Module Expr (T : TermDef).
         | e_pair1 _ _ a => fun pf pf' => e_pair1 (exp_subst i t (eq_rect_exp pf pf' a))
         | e_pair2 _ _ a => fun pf pf' => e_pair2 (exp_subst i t (eq_rect_exp pf pf' a))
       end eq_refl eq_refl.
-
-    (* Lemma exp_subst_neq : forall {n m} u (v : exp n m), e_app (e_abs u) v = exp_subst Fin.F1 v u -> False. *)
-    (* Proof. *)
-    (*   dependent destruction u; simpl; intros v p; try (inversion p; fail). *)
-    (*   destruct (fin_subst v Fin.F1 t) eqn:H. *)
-    (*   + apply eq_fin_subst in H; subst v. admit. *)
-    (*   + inversion p. *)
-    (*   + inversion p; simpl_exist. *)
-    (*     dependent destruction u1; try (simpl in H0; inversion H0; fail). *)
-    (*     dependent destruction t. *)
-    (*     * simpl in H0; rewrite fin_subst_eq in H0. *)
-    (*       rewrite H1 in H0; dependent destruction u2; try (simpl in H0; inversion H0; fail). *)
-    (*       dependent destruction t. *)
-          
-
-
-      
     Reserved Notation "a '===>' b" (at level 60).
+
+    Fixpoint exp_subst_term {n m} (i : Fin.t (S m)) (t : term m) (u : exp n (S m)) : exp n m :=
+      let eq_rect_exp {n m n' m'} (pf : n' = n) (pf' : m' = S m) (x : exp n' m') :=
+          eq_rect n' (fun i => exp i (S m)) (eq_rect m' (fun i => exp n' i) x _ pf') _ pf
+      in
+      match u as u' in exp n' m' return forall pf : n' = n,
+                                        forall pf' : m' = S m,
+                                          exp n m
+      with
+        | e_var n' _ j => fun pf pf' => eq_rect n' (fun i => exp i m) (e_var j) _ pf
+        | e_app _ _ a b => fun pf pf' => e_app (exp_subst_term i t (eq_rect_exp pf pf' a)) (exp_subst_term i t (eq_rect_exp pf pf' b))
+        | e_forall _ _ a => fun pf pf' => e_forall (exp_subst_term (Fin.FS i) (lift_term t) (eq_rect_exp pf (f_equal S pf') a))
+        | e_exists _ m' a b => fun pf pf' => e_exists (term_subst i t (eq_rect m' term a _ pf')) (exp_subst_term i t (eq_rect_exp pf pf' b))
+        | e_ecase _ _ a b => fun pf pf' => e_ecase (exp_subst_term i t (eq_rect_exp pf pf' a)) (exp_subst_term (Fin.FS i) (lift_term t) (eq_rect_exp (f_equal S pf) (f_equal S pf') b))
+        | e_abs _ _ a => fun pf pf' => e_abs (exp_subst_term i t (eq_rect_exp (f_equal S pf) pf' a))
+        | e_tapp _ m' a b => fun pf pf' => e_tapp (exp_subst_term i t (eq_rect_exp pf pf' a)) (term_subst i t (eq_rect m' term b _ pf'))
+        | e_absurd _ _ a => fun pf pf' => e_absurd (exp_subst_term i t (eq_rect_exp pf pf' a))
+        | e_copair1 _ _ a => fun pf pf' => e_copair1 (exp_subst_term i t (eq_rect_exp pf pf' a))
+        | e_copair2 _ _ a => fun pf pf' => e_copair2 (exp_subst_term i t (eq_rect_exp pf pf' a))
+        | e_case _ _ a b c => fun pf pf' => e_case
+                                              (exp_subst_term i t (eq_rect_exp pf pf' a))
+                                              (exp_subst_term i t (eq_rect_exp (f_equal S pf) pf' b))
+                                              (exp_subst_term i t (eq_rect_exp (f_equal S pf) pf' c))
+        | e_tt _ _ => fun _ _ => e_tt
+        | e_pair _ _ a b => fun pf pf' => e_pair (exp_subst_term i t (eq_rect_exp pf pf' a)) (exp_subst_term i t (eq_rect_exp pf pf' b))
+        | e_pair1 _ _ a => fun pf pf' => e_pair1 (exp_subst_term i t (eq_rect_exp pf pf' a))
+        | e_pair2 _ _ a => fun pf pf' => e_pair2 (exp_subst_term i t (eq_rect_exp pf pf' a))
+      end eq_refl eq_refl.
     
+    Reserved Notation "a '===>' b" (at level 60).
+
     Inductive reduction : forall {n m}, exp n m -> exp n m -> Prop :=
     | reduction_beta : forall n m (a : exp (S n) m) b, e_app (e_abs a) b ===> exp_subst Fin.F1 b a
-    (* | reduction_forall : forall n m a b, reduction (t_app (e_forall a) b) (exp_subst Fin.F1 b a) *)
+    | reduction_forall : forall n m (a : exp n (S m)) (b : term m), reduction (e_tapp (e_forall a) b) (exp_subst_term Fin.F1 b a)
     | reduction_absurd : forall n m (a : exp n m) b, e_app (e_absurd a) b ===> e_absurd a
-    (* | reduction_ecase *)
+    | reduction_ecase : forall n m t (a : exp n m) b, e_ecase (e_exists t a) b ===> exp_subst Fin.F1 a (exp_subst_term Fin.F1 t b)
     | reduction_case1 : forall n m (a : exp n m) u v, e_case (e_copair1 a) u v ===> exp_subst Fin.F1 a u
     | reduction_case2 : forall n m (a : exp n m) u v, e_case (e_copair2 a) u v ===> exp_subst Fin.F1 a v
     | reduction_pair1 : forall n m (a : exp n m) b, e_pair1 (e_pair a b) ===> a
@@ -360,7 +555,7 @@ Module Expr (T : TermDef).
     | reduction_context_exists : forall n m (a : exp n m) a' t, a ===> a' -> e_exists t a ===> e_exists t a'
     | reduction_context_ecase_1 : forall n m (a : exp n m) b a', a ===> a' -> e_ecase a b ===> e_ecase a' b
     | reduction_context_ecase_2 : forall n m (a : exp n m) b b', b ===> b' -> e_ecase a b ===> e_ecase a b'
-    | reduction_context_tapp : forall n m (a : exp n (S m)) a' t, a ===> a' -> e_tapp a t ===> e_tapp a' t
+    | reduction_context_tapp : forall n m (a : exp n m) a' t, a ===> a' -> e_tapp a t ===> e_tapp a' t
     | reduction_context_absurd : forall n m (a : exp n m) a', a ===> a' -> e_absurd a ===> e_absurd a'
     | reduction_context_case_1 : forall n m (a : exp n m) b c a', a ===> a' -> e_case a b c ===> e_case a' b c
     | reduction_context_case_2 : forall n m (a : exp n m) b c b', b ===> b' -> e_case a b c ===> e_case a b' c
@@ -401,8 +596,10 @@ Module Expr (T : TermDef).
          | nfv_exists : forall n m t (e : exp n m),
                           nfview e -> nfview_unknown (e_exists t e)
          | nfv_ecase : forall n m (a : exp n m) (b : exp (S n) (S m)),
+                         (forall x y, a = e_exists x y -> False) ->
                          nfview a -> nfview b -> nfview_unknown (e_ecase a b)
-         | nfv_tapp : forall n m (a : exp n (S m)) t,
+         | nfv_tapp : forall n m (a : exp n m) t,
+                        (forall x, a = e_forall x -> False) ->
                         nfview a -> nfview_unknown (e_tapp a t)
          | nfv_copair1 : forall n m (a : exp n m),
                            nfview a -> nfview_unknown (e_copair1 a)
@@ -422,7 +619,7 @@ Module Expr (T : TermDef).
                          (forall x y, a = e_pair x y -> False) ->
                          nfview a -> nfview_unknown (e_pair2 a)
     .
-
+    
     Ltac nf_nfview_helper p := 
       match goal with
         | [ IH : nf ?e -> nfview ?e |- nfview ?e ] =>
@@ -453,11 +650,11 @@ Module Expr (T : TermDef).
       intros n m e; set (e0 := e); dependent induction e;
       (assert (S2 : nfview_unknown e0 -> nf e0);
       [ subst e0; intro;
-        repeat match goal with [ H : _ /\ _ |- _ ] => destruct H end;
+        destruct_pairs;
         try (intros e' H'; inversion H'; fail);
         inversion H; simpl_exist; subst; eauto
       | split; [|exact S2]; subst e0; intro;
-        repeat match goal with [ H : _ /\ _ |- _ ] => destruct H end;
+        destruct_pairs;
         inversion H; simpl_exist; subst;
         try (match goal with
                  [ H : fold_right _ _ _ = _ |- _ ] => destruct ns; [ simpl in H; subst; auto
@@ -477,12 +674,18 @@ Module Expr (T : TermDef).
           inversion H8.
           unfold nf in H3; eapply H3; eauto.
           unfold nf in H0; eapply H0; eauto.
-
         * simpl_forall_list.
           intros e' H'; inversion H'; simpl_exist; subst.
           unfold nf in H2; eapply H2... apply nfv_unknown with (e:=e) (ns:=cons e3 ns)...
           unfold nf in H0; eapply H0; eauto.
-    Qed.     
+    Qed.
+
+    Theorem nfview_app : forall {n m} (a b : exp n m), nfview (e_app a b) -> nfview a.
+    Proof.
+      intros.
+      apply nfview_nf in H.
+      apply nf_nfview. intro. intros. eapply H. eapply reduction_context_app_1. eauto.
+    Qed.
       
 End Expr.
 
@@ -509,8 +712,7 @@ Module NJ (T : TermDef) (TC : TermCongruence(T)).
                          ty_arrow x z ≡ ty_arrow y t
   | te_context_forall : forall {n} {x y : type (S n)},
                           x ≡ y ->
-                          ty_forall x c
-                                    ≡ ty_forall y
+                          ty_forall x ≡ ty_forall y
   | te_context_exists : forall {n} {x y : type (S n)},
                           x ≡ y ->
                           ty_exists x ≡ ty_exists y
@@ -538,64 +740,70 @@ Module NJ (T : TermDef) (TC : TermCongruence(T)).
   Qed.
   
   Definition liftΓ {n m} (Γ : Vector.t (type m) n) : Vector.t (type (S m)) n := Vector.map lift_type Γ.
+
+  Theorem liftΓ_inj : forall {n m} (Γ1 Γ2 : Vector.t (type m) n),
+                        liftΓ Γ1 = liftΓ Γ2 -> Γ1 = Γ2.
+  Proof.
+    induction Γ1; intros; dependent destruction Γ2; auto.
+    simpl in H. inversion H. f_equal; simpl_exist; auto.
+  Qed.
+
+  Hint Immediate liftΓ_inj.
   
   Reserved Notation "Γ '⊢' t '∈' ty" (at level 40).
   
   Inductive has_type : forall {n m : nat}, Vector.t (type m) n -> exp n m -> type m -> Prop :=
-  | p_equiv : forall m n (Γ : Vector.t (type m) n) e ty ty',
-              ty ≡ ty' ->
-              Γ ⊢ e ∈ ty -> Γ ⊢ e ∈ ty'
-  | p_var : forall m n (Γ : Vector.t (type m) n) i,
-            Γ ⊢ e_var i ∈ Vector.nth Γ i
-  | p_app : forall m n (Γ : Vector.t (type m) n) u v s t,
+  | p_var : forall {n m} {Γ : Vector.t (type m) n} i ty,
+              ty ≡ Vector.nth Γ i -> Γ ⊢ e_var i ∈ ty
+  | p_app : forall {n m} {Γ : Vector.t (type m) n} {u v s t ty},
             Γ ⊢ u ∈ ty_arrow s t ->
             Γ ⊢ v ∈ s ->
-            Γ ⊢ e_app u v ∈ t
-  | p_abs : forall m n (Γ : Vector.t (type m) n) e t u,
+            ty ≡ t -> Γ ⊢ e_app u v ∈ ty
+  | p_abs : forall {n m} {Γ : Vector.t (type m) n} {e t u ty},
               (t :: Γ) ⊢ e ∈ u ->
-              Γ ⊢ e_abs e ∈ ty_arrow t u
-  | p_forall : forall m n (Γ : Vector.t (type m) n) e u,
+              ty ≡ ty_arrow t u -> Γ ⊢ e_abs e ∈ ty
+  | p_forall : forall {n m} {Γ : Vector.t (type m) n} {e u ty},
                  (liftΓ Γ) ⊢ e ∈ u ->
-                 Γ ⊢ e_forall e ∈ ty_forall u
-  | p_exists : forall m n (Γ : Vector.t (type m) n) t u p,
+                 ty ≡ ty_forall u -> Γ ⊢ e_forall e ∈ ty
+  | p_exists : forall {n m} {Γ : Vector.t (type m) n} {t u p ty},
                  Γ ⊢ u ∈ type_subst Fin.F1 t p ->
-                 Γ ⊢ e_exists t u ∈ ty_exists p
-  | p_ecase : forall m n (Γ : Vector.t (type m) n) u v p q,
+                 ty ≡ ty_exists p -> Γ ⊢ e_exists t u ∈ ty
+  | p_ecase : forall {n m} {Γ : Vector.t (type m) n} {u v p q ty},
                 Γ ⊢ u ∈ ty_exists p ->
                 (p :: liftΓ Γ) ⊢ v ∈ lift_type q ->
-                Γ ⊢ e_ecase u v ∈ q
-  | p_copair1 : forall m n (Γ : Vector.t (type m) n) u s t,
+                ty ≡ q -> Γ ⊢ e_ecase u v ∈ ty
+  | p_copair1 : forall {n m} {Γ : Vector.t (type m) n} {u s t ty},
                   Γ ⊢ u ∈ s ->
-                  Γ ⊢ e_copair1 u ∈ ty_copair s t
-  | p_copair2 : forall m n (Γ : Vector.t (type m) n) v s t,
+                  ty ≡ ty_copair s t -> Γ ⊢ e_copair1 u ∈ ty
+  | p_copair2 : forall {n m} {Γ : Vector.t (type m) n} {v s t ty},
                   Γ ⊢ v ∈ t ->
-                  Γ ⊢ e_copair2 v ∈ ty_copair s t
-  | p_case : forall m n (Γ : Vector.t (type m) n) a b u v1 v2 t,
+                  ty ≡ ty_copair s t -> Γ ⊢ e_copair2 v ∈ ty
+  | p_case : forall {n m} {Γ : Vector.t (type m) n} {a b u v1 v2 t ty},
                Γ ⊢ u ∈ ty_copair a b ->
                (a :: Γ) ⊢ v1 ∈ t ->
                (b :: Γ) ⊢ v2 ∈ t ->
-               Γ ⊢ e_case u v1 v2 ∈ t
-  | p_pair : forall m n (Γ : Vector.t (type m) n) u v s t,
+               ty ≡ t -> Γ ⊢ e_case u v1 v2 ∈ ty
+  | p_pair : forall {n m} {Γ : Vector.t (type m) n} {u v s t ty},
                Γ ⊢ u ∈ s ->
                Γ ⊢ v ∈ t ->
-               Γ ⊢ e_pair u v ∈ ty_pair s t
-  | p_pair1 : forall m n (Γ : Vector.t (type m) n) u s t,
+               ty ≡ ty_pair s t -> Γ ⊢ e_pair u v ∈ ty
+  | p_pair1 : forall {n m} {Γ : Vector.t (type m) n} {u s t ty},
                   Γ ⊢ u ∈ ty_pair s t ->
-                  Γ ⊢ e_pair1 u ∈ s
-  | p_pair2 : forall m n (Γ : Vector.t (type m) n) u s t,
+                  ty ≡ s -> Γ ⊢ e_pair1 u ∈ ty
+  | p_pair2 : forall {n m} {Γ : Vector.t (type m) n} {u s t ty},
                   Γ ⊢ u ∈ ty_pair s t ->
-                  Γ ⊢ e_pair2 u ∈ t
-  | p_absurd : forall m n (Γ : Vector.t (type m) n) e t,
+                  ty ≡ t -> Γ ⊢ e_pair2 u ∈ ty
+  | p_absurd : forall {n m} {Γ : Vector.t (type m) n} {e t ty},
                  Γ ⊢ e ∈ ty_bottom ->
-                 Γ ⊢ e_absurd e ∈ t
-  | p_tt : forall m n (Γ : Vector.t (type m) n),
-             Γ ⊢ e_tt ∈ ty_top
+                 ty ≡ t -> Γ ⊢ e_absurd e ∈ ty
+  | p_tt : forall {n m} {Γ : Vector.t (type m) n} {ty},
+             ty ≡ ty_top -> Γ ⊢ e_tt ∈ ty
                where "Γ '⊢' t '∈' ty" := (has_type Γ t ty).
+    
+  Definition is_typable {n m : nat} (e : exp n m) := sigma Γ ty, Γ ⊢ e ∈ ty.
+  Definition is_provable {n : nat} (ty : type n) := sigma {e : exp O n}, [] ⊢ e ∈ ty.
+  Definition is_provable_nf {n : nat} (ty : type n) := (sigma {e : exp O n}, nf e * ([] ⊢ e ∈ ty))%type.
   
-  Definition is_typable {n m : nat} (e : exp n m) := exists Γ ty, Γ ⊢ e ∈ ty.
-  Definition is_provable {n : nat} (ty : type n) := exists {e : exp O n}, [] ⊢ e ∈ ty.
-  Definition is_provable_nf {n : nat} (ty : type n) := exists {e : exp O n}, nf e /\ [] ⊢ e ∈ ty.
-
 End NJ.
 
 Module Ex1Term <: TermDef.
@@ -605,7 +813,14 @@ Module Ex1Term <: TermDef.
   | s_plus
   | s_equal
   .
+
   Definition symbol := symbol_.
+
+  Theorem eq_symbol_dec : forall (s s' : symbol), {s = s'} + {s <> s'}.
+  Proof.
+    decide equality.
+  Qed.
+    
   Fixpoint arity s :=
     match s with
       | s_zero => 0
@@ -685,29 +900,29 @@ Module Q1.
   Theorem Q1a : is_provable (@ty_term 0 (t_term s_equal [t_term s_plus [t_of_nat 2; t_of_nat 3]; t_of_nat 5])).
   Proof with eauto.
     eexists e_tt.
-    eapply p_equiv; [|constructor].
+    constructor.
     simpl_equiv.
   Qed.
   
   Theorem Q1b : is_provable (@ty_forall 0 (ty_term (t_term s_equal [t_term s_plus [t_of_nat 2; t_var Fin.F1]; t_term s_plus [t_of_nat 1; t_term s_plus [t_of_nat 1; t_var Fin.F1]]]))).
   Proof with eauto.
     eexists (e_forall e_tt).
-    eapply p_equiv; [|repeat constructor].
-    simpl_equiv.
+    repeat (simpl_equiv || econstructor).
   Qed.
   
   Theorem Q1c : is_provable (@ty_arrow 0 (ty_term (t_term s_equal [t_term s_plus [t_of_nat 1; t_of_nat 1]; t_term s_zero []])) (ty_term (t_term s_equal [t_term s_plus [t_of_nat 16; t_of_nat 64]; t_of_nat 42]))).
   Proof with eauto.
-    eexists. constructor.
-    apply p_absurd. eapply p_equiv; [|apply p_var with (i:=Fin.F1)]. simpl.
-    simpl_equiv.
+    eexists.
+    eapply p_abs; [eapply p_absurd;[apply p_var with (i:=Fin.F1)|]|].
+    simpl_equiv. simpl_equiv.
+    eapply te_context_arrow. simpl_equiv. eapply te_refl.
   Qed.
   
   Theorem Q1d : is_provable (@ty_forall 0 (ty_arrow (ty_term (t_term s_equal [t_var Fin.F1; t_of_nat 2])) (ty_term (t_term s_equal [t_term s_plus [t_of_nat 1; t_var Fin.F1]; t_of_nat 3])))).
   Proof with eauto.
-    eexists. do 2 constructor.
-    eapply p_equiv; [|apply p_var with (i:=Fin.F1)]. simpl.
-    simpl_equiv.
+    eexists.
+    eapply p_forall;[eapply p_abs;[apply p_var with (i:=Fin.F1)|]|];
+    repeat simpl_equiv.
   Qed.
 
 End Q1.
@@ -721,6 +936,8 @@ Module Ex2Term <: TermDef.
   | s_n
   .
   Definition symbol := symbol_.
+  Theorem eq_symbol_dec : forall (s s' : symbol), {s=s'}+{s<>s'}.
+  Proof. decide equality. Qed.
   Fixpoint arity s :=
     match s with
       | s_zero => 0
@@ -777,20 +994,20 @@ Module Q2.
                                          )
                            ).
   Proof.
-    eexists. do 3 constructor; simpl.
-    + eapply p_equiv; [ eapply te_sym; eapply te_term; eapply c_n
-                      | eapply p_copair2; eapply p_exists; eapply p_pair; simpl ].
-      eapply p_equiv; [ eapply te_sym; eapply te_term; eapply c_refl | eapply p_tt ].
-      eapply p_equiv; [ | eapply p_var with (i:=Fin.F1) ].
-      simpl; eapply te_refl.
-    + eapply p_case; [ eapply p_equiv; [| eapply p_var with (i:=Fin.F1) ]
-                     | 
-                     | eapply p_pair2; eapply p_ecase; [|]
-                     ]; simpl.
-      eapply te_term; eapply c_n.
-      eapply p_absurd; eapply p_equiv; [| eapply p_var with (i:=Fin.F1) ]. simpl; eapply te_term; eapply c_neq_0.
-      simpl. eapply p_equiv; [|eapply p_var with (i:=Fin.F1)]. simpl. eapply te_refl.
-      simpl. eapply p_equiv; [|eapply p_var with (i:=Fin.F1)]. simpl.
+    (* eexists. do 3 constructor; simpl. *)
+    (* + eapply p_equiv; [ eapply te_sym; eapply te_term; eapply c_n *)
+    (*                   | eapply p_copair2; eapply p_exists; eapply p_pair; simpl ]. *)
+    (*   eapply p_equiv; [ eapply te_sym; eapply te_term; eapply c_refl | eapply p_tt ]. *)
+    (*   eapply p_equiv; [ | eapply p_var with (i:=Fin.F1) ]. *)
+    (*   simpl; eapply te_refl. *)
+    (* + eapply p_case; [ eapply p_equiv; [| eapply p_var with (i:=Fin.F1) ] *)
+    (*                  |  *)
+    (*                  | eapply p_pair2; eapply p_ecase; [|] *)
+    (*                  ]; simpl. *)
+    (*   eapply te_term; eapply c_n. *)
+    (*   eapply p_absurd; eapply p_equiv; [| eapply p_var with (i:=Fin.F1) ]. simpl; eapply te_term; eapply c_neq_0. *)
+    (*   simpl. eapply p_equiv; [|eapply p_var with (i:=Fin.F1)]. simpl. eapply te_refl. *)
+    (*   simpl. eapply p_equiv; [|eapply p_var with (i:=Fin.F1)]. simpl. *)
   Admitted.
 
 End Q2.
@@ -799,8 +1016,9 @@ Module Ex3Term <: TermDef.
   Inductive symbol_ :=
   | s_p
   .
-  
   Definition symbol := symbol_.
+  Theorem eq_symbol_dec : forall (s s' : symbol), {s=s'}+{s<>s'}.
+  Proof. decide equality. Qed.
   Fixpoint arity s :=
     match s with
       | s_p => 0
@@ -828,11 +1046,11 @@ Module Q3.
   Theorem Q3 : @is_provable 0 ty_bottom.
   Proof.
     eexists.
-    eapply p_app; eapply p_abs; eapply p_app; eapply p_equiv; try eapply p_var with (i:=Fin.F1).
-    simpl; eapply te_refl.
-    simpl; eapply te_sym; eapply te_term; eapply c_p.
-    simpl; eapply te_term; eapply c_p.
-    simpl; eapply te_refl.
+    eapply p_app; try eapply p_abs; try eapply p_app; try eapply p_var with (i:=Fin.F1);
+    simpl; try eapply te_refl.
+    eapply te_context_arrow; try apply te_refl.
+    eapply te_term. eapply c_p.
+    eapply te_term. eapply c_p.
   Qed.
     
 End Q3.
@@ -857,40 +1075,109 @@ Module Q4(T:TermDef)(TC:TermCongruence(T)).
   .
 
   Definition sans_confusion := forall n p q, p ≡ q -> @weak_equiv n p q.
+
+  Ltac simpl_fold :=
+    repeat match goal with
+               [ H1 : context[fold_right _ _ nil] |- _ ] => simpl in H1; subst
+           end.
+
+  Ltac simpl_nf :=
+    match goal with
+      | [ H : nfview _ |- _ ] =>
+        inversion H; simpl_exist; subst;
+        try (solve by inversion);
+        match goal with
+            [ H0 : Forall nfview ?ns |- _ ] =>
+            destruct ns; simpl;
+            [ clear H H0
+            | solve by inversion
+            ]; simpl_fold
+        end
+      | [ H : nfview _ |- _ ] =>
+        inversion H; simpl_exist; subst;
+        [ match goal with
+              [ H0 : Forall nfview ?ns |- _ ] =>
+              destruct ns; simpl_fold; solve by inversion
+          end
+        |]
+      | [ H : nfview (e_app _ _) |- _ ] => apply nfview_app in H
+    end.
+
+  Ltac simpl_empty_nf :=
+    repeat match goal with
+             | [ H : ?x = ?x -> _ |- _ ] =>
+               let H0 := fresh "H" in
+               assert (H0 : x = x); [ reflexivity | specialize (H H0); clear H0 ]
+             | [ H : 1 = 0 -> _ |- _ ] => clear H
+             | [ H : 0 = 1 -> _ |- _ ] => clear H
+             | [ H : ?a, H0 : ?a -> ?b |- _ ] => specialize (H0 H)
+           end.
   
-  Theorem sans_confusion_coherent : sans_confusion -> @is_provable_nf 0 ty_bottom -> False.
-  Proof with simpl_exist; subst; auto.
-    unfold sans_confusion.
-    intros H p. destruct p as [u [nf p]].
-    dependent induction p...
-    + assert (H1 := H _ _ _ H0).
-      inversion H1; subst;
-      try (apply Fin.case0; auto; fail)...
-    + apply Fin.case0...
-    + admit.
-    + dependent induction p2; subst;
-      try (apply Fin.case0; auto; fail); simpl in *...
-      admit.
-      admit.
-      eapply nf0; constructor; apply reduction_refl.
-      admit.
-      admit.
-      admit.
-      admit.
-      admit.
-    + 
-      
-      
-    
+  Lemma empty_nf : sans_confusion ->
+                   (forall n m Γ (e : exp n m) ty (P : Γ ⊢ e ∈ ty),
+                      n = 0 -> m = 0 -> nfview e ->
+                      (forall x, e <> e_absurd x) /\
+                      (forall x y, e <> e_app x y) /\
+                      (forall x y, e <> e_tapp x y) /\
+                      (forall x, e <> e_pair1 x) /\
+                      (forall x, e <> e_pair2 x) /\
+                      (forall x y, e <> e_ecase x y) /\
+                      (forall x y z, e <> e_case x y z) /\
+                      ty <> ty_bottom
+                   ).
+  Proof.
+    Ltac solver :=
+      match goal with
+        | [ H : sans_confusion, H0 : _ ≡ _ |- _ ] =>
+          (apply H in H0; try (inversion H0; simpl_exist; subst;
+                               try (apply Fin.case0; trivial; fail);
+                               try (unfold not; intro A; inversion A; fail);
+                               fail))
+        | [ H0 : appcontext[?x = ?x -> False] |- _ ] => (eapply H0; eauto)
+        | [ H0 : appcontext[?x _ = ?x _ -> False] |- _ ] => (eapply H0; eauto)
+        | [ H0 : appcontext[?x _ _ = ?x _ _ -> False] |- _ ] => (eapply H0; eauto)
+        | [ H0 : appcontext[?x _ _ _ = ?x _ _ _ -> False] |- _ ] => (eapply H0; eauto)
+      end.
+
+    intros H n m Γ e ty P.
+    induction P; intros; subst;
+    repeat constructor;
+    try (intros; unfold not; intro A; inversion A; fail);
+    try (apply Fin.case0; trivial; fail);
+    solver; unfold not in *;
+    try (exfalso; simpl_nf; try inversion H6; simpl_exist;
+         simpl_empty_nf; destruct_pairs;
+         match goal with
+           | [ P : has_type Γ _ _ |- _ ] =>
+             inversion P; simpl_exist;
+           try (apply Fin.case0; trivial; fail);
+           repeat solver
+         end; fail
+        );
+    try ( exfalso; inversion H3; simpl_exist; subst;
+          destruct ns; simpl_fold;
+          [ inversion H6
+          | destruct ns; inversion H1; simpl_exist; subst; simpl_forall_list;
+            apply nfview_app in H3; simpl_empty_nf; destruct_pairs;
+            [ inversion H6; simpl_exist; subst;
+              try (apply Fin.case0; auto; fail);
+              try (inversion P1; simpl_exist; subst; try solver; fail);
+              try solver
+            | solver
+            ]
+          ]; fail).
+  Qed.
+
+  Theorem sans_confusion_coherent : sans_confusion ->
+                                    forall (u : exp 0 0), nf u -> [] ⊢ u ∈ ty_bottom -> False.
+  Proof.
+    intros H u nf p.
+    apply nf_nfview in nf.
+    assert (P := empty_nf H _ _ _ _ _ p).
+    assert (0=0). reflexivity.
+    specialize (P H0 H0 nf).
+    destruct_pairs.
+    apply H8; auto.
+  Qed.
+  
 End Q4.
-
-
-
-
-
-
-
-
-
-
-Module Q5
